Prove n^2 lower bound for the time complexity of fibonacci!
This commit removes many lemmas that were unecessary for the fib lower bound proof.
Many of these will return for the proof of n^2 as an upper bound as well.

fib/fib_iter.v
@@ -84,6 +84,19 @@ Fixpoint fib_iter_time_lb (n:nat) :=
       end
   end.
 
+Lemma relate_fib_iter_fib_iter_loop :
+  forall n,
+    1 < n ->
+    fib_iter_time_lb n = 1 + fib_iter_loop_time_lb (n-1) 0 1.
+Proof.
+  intros.
+  destruct n. inversion H.
+  destruct n. intuition.
+  unfold fib_iter_time_lb.
+  replace (S (S n) - 1) with (S n); try omega.
+Qed.  
+  
+
 Fixpoint fib_iter_time_ub (n:nat) :=
   match n with
     | O => 1
@@ -149,49 +162,12 @@ Proof.
   auto.
 Qed.
 
-Lemma plus_two_fibs_time_upper_bound :
-  forall n, plus_two_fibs_time n <= n + 4.
-Proof.
-  intros.
-  unfold plus_two_fibs_time.
-  unfold plus_time_lb.
-  apply (le_trans
-           (plus_cin_time_lb (fib n) (fib (n + 1))+1)
-           (plus_cin_time_lb (fib (n+1)) (fib (n + 1))+1)).
-  rewrite plus_cin_time_lb_symmetric.
-  apply plus_le_compat; auto.
-  apply plus_cin_time_lb_right_arg_grows.
-  apply fib_monotone.
-  omega.
-  replace (plus_cin_time_lb (fib (n + 1)) (fib (n + 1))+1) with
-          (plus_time_lb (fib (n + 1)) (fib (n + 1))).
-  rewrite plus_time_lb_below_log_nn.
-  replace (n+4) with ((n+2)+2);[|omega].
-  apply plus_le_compat; auto.
-  eapply le_trans.
-  apply fib_log_upper_bound. omega.
-  unfold plus_time_lb. auto.
-Qed.  
   
 Fixpoint fib_iter_loop_time_lb2 fuel n :=
   match fuel with
     | 0 => 1
     | S fuel' => plus_two_fibs_time n + 
                  fib_iter_loop_time_lb2 fuel' (n+1) + 1
-  end.
-
-Fixpoint fib_iter_loop_time_lb22 fuel n :=
-  match fuel with
-    | 0 => 1
-    | S fuel' => plus_two_fibs_time (n+fuel') +
-                 fib_iter_loop_time_lb22 fuel' n + 1
-  end.
-
-Fixpoint fib_iter_loop_time_lb2_rev fuel n :=
-  match fuel with
-    | 0 => 1
-    | S fuel' => plus_two_fibs_time n +
-                 fib_iter_loop_time_lb2_rev fuel' (pred n) + 1
   end.
 
 
@@ -231,22 +207,6 @@ Proof.
   rewrite sum_constant with (k:=fuel-1); try omega.
 Qed.
 
-Lemma fib_iter_loop_lb2_upper_bound1 :
-  forall fuel n,
-    0 < fuel ->
-    fib_iter_loop_time_lb2 fuel n <=
-    1 + fuel + sum 0 (fuel - 1) (const (plus_two_fibs_time (n+fuel))).
-Proof.
-  intros.
-  rewrite fib_iter_loop_lb2_sum3; auto.
-  apply plus_le_compat; auto.
-  apply sum_preserves_order_in_range.
-  intros.
-  unfold const.  
-  apply plus_two_fibs_time_monotone.
-  apply plus_le_compat; auto.
-  omega.
-Qed.
   
 Lemma fib_iter_loop_lb2_lower_bound1 :
   forall fuel n,
@@ -304,22 +264,6 @@ Proof.
   apply fib_iter_loop_lb2_lower_bound1. auto.
 Qed.
 
-
-Lemma fib_iter_loop_lb2_closed_upper_bound :
-  forall fuel n,
-    0 < fuel ->
-    fib_iter_loop_time_lb2 fuel n <=
-    1 + fuel + fuel*plus_two_fibs_time (n+fuel).
-Proof.  
-  intros.
-  eapply le_trans.
-  apply fib_iter_loop_lb2_upper_bound1; auto.
-  apply plus_le_compat; auto.
-  unfold const.
-  rewrite sum_constant with (k:=fuel-1); try omega.
-  replace (fuel - 1 + 1 ) with fuel; try omega.
-Qed.
-
 Lemma fib_iter_loop_time_lb2_closed_lower_bound :
   forall fuel n,
     4 < fuel ->
@@ -349,35 +293,6 @@ Proof.
   apply fib_iter_loop_lb2_lower_bound2; auto.
 Qed.  
   
-  
-Lemma fib_iter_loop_time_lb_monotone :
-  forall a b n n',
-    n <= n' ->
-    fib_iter_loop_time_lb n a b <= fib_iter_loop_time_lb n' a b.
-Proof.
-  intros.
-  apply (well_founded_ind
-           lt_wf
-           (fun n => forall a b n', n<=n'-> fib_iter_loop_time_lb n a b <= fib_iter_loop_time_lb n' a b));[|auto].
-  intros.
-  destruct x.
-  simpl.
-  inversion H1.
-  simpl.
-  auto.
-  simpl.
-  omega.
-  inversion H1.
-  simpl.
-  auto.
-  simpl.
-  apply plus_le_compat; auto.
-  apply plus_le_compat.
-  auto.
-  apply H0.
-  auto.
-  omega.
-Qed.
 
 Lemma fib_iter_loop_lb12 : 
   forall n steps_taken,
@@ -404,41 +319,6 @@ Proof.
 Qed.
 
 
-Lemma fib_iter_loop_time_lb2_grows:
-  forall fuel n, 
-    fib_iter_loop_time_lb2 fuel n <= fib_iter_loop_time_lb2 fuel (n + 1).
-Proof.
-  intros fuel.
-  induction fuel.
-  intros; simpl;omega.
-  intros n.
-  unfold fib_iter_loop_time_lb2; fold fib_iter_loop_time_lb2.
-  repeat (apply plus_le_compat); auto.
-  clear IHfuel.
-  rewrite plus_cin_time_lb_symmetric at 1.
-  apply plus_cin_time_lb_right_arg_grows.
-  apply fib_monotone.
-  omega.
-Qed.
-
-Lemma fib_iter_loop_time_lb2_lower_bound :
-  forall fuel n,
-    fuel*(plus_two_fibs_time n + 1) <=  fib_iter_loop_time_lb2 fuel n. 
-Proof.
-  intro fuel.
-  induction fuel.
-  intros.
-  simpl.
-  auto.
-  intros.
-  simpl.
-  rewrite <- plus_assoc. rewrite <- plus_assoc.
-  apply plus_le_compat.
-  auto. rewrite plus_comm. apply plus_le_compat; auto.
-  eapply le_trans.
-  apply IHfuel.
-  apply fib_iter_loop_time_lb2_grows.
-Qed.
 
 
 Lemma div2_inc1 : forall n, div2 n <= div2 (S n).
@@ -476,7 +356,7 @@ Proof.
   apply div2_inc1.
   auto.
 Qed.  
-  
+
 Lemma plus_two_fibs_time_below :
   forall n, 4<=n -> n <= 4*plus_two_fibs_time n.
 Proof.
@@ -529,215 +409,6 @@ Proof.
   omega.
 Qed.
   
-Lemma plus_time_lb_big_oh_plus_cin_time_lb :
-  big_oh (fun n : nat => plus_time_lb (fib n) (fib n))
-         (fun n : nat => plus_cin_time_lb (fib n) (fib n)).
-Proof.
-  unfold plus_time_lb.
-  exists 1 2.
-  intros n LE.
-  apply plus_cin_time_lb_growth.
-Qed.
-
-Lemma plus_two_fibs_time_lb :
-  big_oh (fun n => n) plus_two_fibs_time.
-Proof.
-  apply (big_oh_trans (fun n => n) div2).
-  exists 2 4.
-  intros n LT.
-  destruct n. intuition.
-  destruct n. intuition.
-  clear LT.
-  apply (well_founded_ind lt_wf (fun n => S (S n) <= 4 * div2 (S (S n)))).
-  clear n; intros n IND.
-  destruct n.
-  simpl; auto.
-  destruct n.
-  simpl; auto.
-  replace (div2 (S (S (S (S n))))) with (S (div2 (S (S n))));[|simpl div2;auto].
-  replace (S (div2 (S (S n)))) with (div2 (S (S n)) + 1);[|omega].
-  rewrite mult_plus_distr_l.
-  rewrite mult_1_r.
-  apply (le_trans (S (S (S (S n)))) (S (S n) + 4)).
-  omega.
-  apply plus_le_compat; auto.
-
-  apply (big_oh_trans div2 (fun n => (plus_cin_time_lb (fib n) (fib (n + 1))))).
-  apply (big_oh_trans div2 (fun n => (plus_cin_time_lb (fib n) (fib n)))).
-  apply (big_oh_trans div2 (fun n => (cl_log (2 * fib n)))).
-  apply (big_oh_trans div2 (fun n => (cl_log (pow 2 (div2 n))))).
-  
-  exists 0 1.
-  intros n _; rewrite mult_1_l.
-  rewrite pow2_log.
-  omega.
-
-  exists 1 1.
-  intros n LT. destruct n. intuition.
-  rewrite mult_1_l.
-  apply cl_log_monotone.
-  apply fib_lower_bound.
-
-  apply (big_oh_trans (fun n => cl_log (2 * fib n))
-                      (fun n => cl_log (fib n))).
-  apply cl_log_big_oh_double.
-
-  apply (big_oh_trans (fun n => cl_log (fib n))
-                      (fun n => plus_time_lb (fib n) (fib n))).
-  exists 0 1.
-  intros n _.
-  rewrite mult_1_l.
-  apply log_below_plus_time_nn.
-
-  apply plus_time_lb_big_oh_plus_cin_time_lb.
-
-  exists 0 1.
-  intros n _.
-  rewrite mult_1_l.
-  apply plus_cin_time_lb_right_arg_grows.
-  apply fib_monotone; omega.
-
-  exists 0 1.
-  intros n _.
-  unfold plus_two_fibs_time.
-  unfold plus_time_lb.
-  omega.
-Qed.
-
-Fixpoint fib_iter_loop_time_lb3 fuel n :=
-  match fuel with
-    | 0 => 1
-    | S fuel' => n +
-                 fib_iter_loop_time_lb3 fuel' (n+1) + 1
-  end.
-
-Lemma fib_iter_loop_time_lb3_Sn :
-  forall fuel n,
-    fib_iter_loop_time_lb3 fuel (S n) = fib_iter_loop_time_lb3 fuel n + fuel.
-Proof.
-  intro fuel.
-  apply (well_founded_ind
-           lt_wf
-           (fun fuel => forall n,  fib_iter_loop_time_lb3 fuel (S n) = fib_iter_loop_time_lb3 fuel n + fuel)).
-  intros.
-  destruct x.
-  simpl. auto.
-  simpl.
-  rewrite H; auto.
-  omega.
-Qed.
-
-Lemma fib_iter_loop_time_lb3_mono_2 :
-  forall fuel, monotone (fib_iter_loop_time_lb3 fuel).
-  intros.
-  unfold monotone.
-  induction fuel.
-  intros.
-  simpl. auto.
-  intros.
-  simpl.
-  apply plus_le_compat;auto.
-  apply plus_le_compat;auto.
-  apply IHfuel.
-  apply plus_le_compat;auto.
-Qed.
-
-Lemma closed_form_fib_iter_loop_time_lb3 :
-  forall n,
-    fib_iter_loop_time_lb3 n 0 = div2 (n*(n+1)) + 1.
-Proof.
-intros.
-induction n.
-simpl. auto.
-simpl fib_iter_loop_time_lb3.
-rewrite fib_iter_loop_time_lb3_Sn.
-rewrite IHn.
-destruct (even_odd_dec n).
-assert (even (S n +1 )).
-simpl.
-constructor.
-replace (n+1) with (S n);[|omega].
-constructor.
-auto.
-rewrite even_div_product; auto.
-replace (S n * (S n + 1)) with ((S n + 1) * S n);[|rewrite mult_comm;auto].
-rewrite even_div_product; auto.
-replace (S n + 1) with (S (S n));[|omega].
-simpl.
-replace (n+1) with (S n);[|omega].
-omega.
-replace (n+1) with (S n);[|omega].
-replace (n* S n) with (S n * n);[|rewrite mult_comm;auto].
-rewrite even_div_product;[|constructor;auto].
-rewrite even_div_product;[|constructor;auto].
-replace (S n + 1) with (n+2);[|omega].
-rewrite mult_plus_distr_l.
-replace 2 with (1+1);[|omega].
-rewrite mult_plus_distr_l.
-rewrite mult_1_r.
-replace  (div2 (S n) + div2 (S n)) with (S n).
-omega.
-replace (S n) with (double (div2 (S n))) at 1.
-auto.
-apply eq_sym.
-apply even_double.
-constructor.
-auto.
-Qed.
-
-Lemma fib_iter_loop_time_lb3_full_closed_form :
-  forall n m,
-    fib_iter_loop_time_lb3 n m = div2(n*(n+1)) + 1 + n*m.
-Proof.
-  intros.
-  generalize dependent n.
-  induction m.
-  intros.
-  rewrite mult_0_r.
-  rewrite plus_0_r.
-  apply closed_form_fib_iter_loop_time_lb3.
-  intros.
-  rewrite fib_iter_loop_time_lb3_Sn.
-  rewrite IHm.
-  replace (S m) with (m + 1);[|omega].
-  rewrite mult_plus_distr_l.
-  rewrite mult_plus_distr_l.
-  rewrite plus_assoc.
-  omega.
-Qed.
-
-Lemma fib_iter_loop_time_lb3_sq : 
-  exists n,
-    forall n',
-      n <= n' ->
-      big_oh (fun n => n*n) (fun fuel => fib_iter_loop_time_lb3 fuel n').
-Proof.
-  exists 0.
-  intros.
-  exists 0.
-  exists 2.
-  intros.
-  apply (le_trans (n*n)
-                  (2*fib_iter_loop_time_lb3 n 0)).
-  rewrite closed_form_fib_iter_loop_time_lb3.
-  rewrite mult_plus_distr_l.
-  simpl.
-  rewrite plus_0_r.
-  replace (div2 (n * (n + 1)) + div2 (n * (n + 1))) with (n*(n+1)).
-  rewrite mult_plus_distr_l.
-  omega.
-  apply even_double.
-  destruct (even_odd_dec n).
-  apply even_mult_l.
-  auto.
-  apply even_mult_r.
-  replace (n+1) with (S n);[|omega].
-  constructor.
-  auto.
-  apply mult_le_compat;auto.
-  apply  fib_iter_loop_time_lb3_mono_2.
-  auto.
-Qed.
 
 Lemma mult_cancel_l :
   forall m n p,
@@ -783,203 +454,69 @@ Proof.
   omega.
 Qed.
   
-Lemma fib_iter_loop_lb23 : 
-  exists n,
-    forall n',
-      n <= n' ->
-      big_oh (fun fuel => fib_iter_loop_time_lb3 fuel n')
-             (fun fuel => fib_iter_loop_time_lb2 fuel n').
+
+Lemma n_squared_big_O_fib_iter_time_lb:
+  big_oh (fun n => n*n) fib_iter_time_lb.
 Proof.
-  
-  exists 0.
-  intros.
-  exists 8.
+  exists 10.
   exists 64.
   intros.
-  rewrite fib_iter_loop_time_lb3_full_closed_form.
-  apply (le_trans (div2 (n * (n + 1)) + 1 + n * n')
-                  (n*(n+1)+1+n*n')).
-  repeat apply plus_le_compat;auto.
-  assert ( div2 (n * (n + 1)) < n * (n + 1)).
-  apply lt_div2.
-  inversion H0. simpl. omega.
-  compute. omega. omega.
+  rewrite relate_fib_iter_fib_iter_loop; try omega.
   rewrite mult_plus_distr_l. rewrite mult_1_r.
-  replace (n * n + n + 1 + n * n') with (1 + n + n*n' + n*n); try omega.
-  apply (le_trans (1 + n + n*n' + n*n)
-                  (64*(1 + n + (div2 n)*(plus_two_fibs_time (n' + div2 n))))).
-  
-  repeat (rewrite mult_plus_distr_l).
-  rewrite mult_1_r.
-  rewrite <- plus_assoc.
-  apply plus_le_compat. omega.
-  rewrite mult_assoc.
-  replace 64 with (16*4); try omega.
-  replace (16 * 4 * div2 n * plus_two_fibs_time (n' + div2 n))
-          with
-          (16 * div2 n * (4 * plus_two_fibs_time (n' + div2 n))).
-  apply (le_trans
-           ( n * n' + n * n)
-           (16*div2 n * (n'+ div2 n))).
-  
-  replace 16 with (4*4); try omega.
-  apply (le_trans  (n * n' + n * n)
-                   (4*n*(n'+div2 n))).
-
-  rewrite mult_plus_distr_l.
-  apply plus_le_compat.
-  apply mult_le_compat; auto. omega.
-
-  replace (4*n) with (n*4).  
-  repeat (rewrite <- mult_assoc).
-  apply mult_le_compat_l; auto.
-  apply mult_4_div2. omega.
-  omega.
-  repeat (rewrite <- mult_assoc).
-  apply mult_le_compat; auto.
-  rewrite mult_assoc.
-  apply mult_le_compat; auto.
-  apply mult_4_div2. omega.
-  apply mult_le_compat; auto.
-  apply plus_two_fibs_time_below.
-  rewrite <- plus_0_l at 1. apply plus_le_compat. auto.
-  replace 4 with (div2 8);[|compute; auto].
-  apply div2_monotone.
-  auto.
-  repeat (rewrite <- mult_assoc).
-  apply mult_cancel_l. omega.
-  repeat (rewrite mult_assoc).
-  apply mult_cancel_r.
-  assert (plus_two_fibs_time 4 <= plus_two_fibs_time (n' + div2 n)).
-  apply plus_two_fibs_time_monotone.
-  rewrite <- plus_0_l at 1. apply plus_le_compat. auto.
-  replace 4 with (div2 8);[|compute;auto].
-  apply div2_monotone. auto.
-  replace (plus_two_fibs_time 4) with 4 in H1;[|compute;auto].
-  omega. omega.
-  apply mult_le_compat;auto.
-  apply fib_iter_loop_time_lb2_closed_lower_bound. omega.
+   replace 0 with (fib 0) at 4;[|simpl; auto].
+   replace 1 with (fib 1) at 4;[|simpl;auto].
+   rewrite fib_iter_loop_lb12.
+   apply (le_trans
+            (n*n)
+            (64 + 64*(1+ (n-1) + (div2 (n-1)*(plus_two_fibs_time (0+div2 (n-1)))))));
+     [|apply plus_le_compat;auto;
+      apply mult_le_compat;auto;
+      apply fib_iter_loop_time_lb2_closed_lower_bound;
+      omega].
+   rewrite plus_0_l.
+   remember (n-1) as N.
+   replace n with (N+1);[|omega].
+   repeat (rewrite mult_plus_distr_l).
+   repeat (rewrite mult_plus_distr_r).
+   repeat (rewrite plus_assoc).
+   repeat (rewrite mult_1_r).
+   repeat (rewrite mult_1_l).
+   replace ( N * N + N + N + 1) with (N * N + 2*N + 1);[|omega].
+   apply (le_trans
+            (N * N + 2 * N + 1)
+            (64 + 64 + 64 * N + 16 * (div2 N * (div2 N))));
+     [|apply plus_le_compat;auto;
+       replace 64 with (16*4);[|omega];
+       repeat (rewrite <- mult_assoc);
+       apply mult_le_compat;auto;
+       replace ((div2 N * plus_two_fibs_time (div2 N))) with
+       ((plus_two_fibs_time (div2 N) * div2 N));[|apply mult_comm];
+       rewrite mult_assoc;
+       apply mult_le_compat;auto;
+       apply plus_two_fibs_time_below;
+       replace 4 with (div2 8);[|simpl;auto];
+       apply div2_monotone;
+       omega].
+   apply (le_trans
+            (N * N + 2 * N + 1)
+            (64 + 64 + 64 * N + N*N)).
+   omega.
+   apply plus_le_compat; auto.
+   rewrite  mult_assoc.
+   replace (16*div2 N) with (div2 N * 16);[|apply mult_comm].
+   replace 16 with (4*4);[|omega].
+   rewrite mult_assoc.
+   replace (div2 N * 4) with (4*div2 N);[|apply mult_comm].
+   replace (4 * div2 N * 4 * div2 N) with ((4*div2 N)*(4*div2 N));
+     [|repeat (rewrite mult_assoc); auto].
+   apply mult_le_compat.
+   apply mult_4_div2. omega.
+   apply mult_4_div2. omega.
 Qed.
-
-Lemma fib_iter_time_lb_big_oh_fib_iter_loop_time_lb : 
-  big_oh (fun n => fib_iter_loop_time_lb n 0 1) fib_iter_time_lb.
-Admitted.
-(* this is likely true. *)
-
-Lemma fib_iter_loop_last_arg_invariant :
-  forall fb, 
-    exists X, 
-      forall n,
-        8 < n ->
-        fib_iter_loop_time_lb2 n fb <= X * fib_iter_loop_time_lb2 n 0.
-Proof.
-  intros.
-  exists (64*(1+fb)).
-  intros.
-  eapply le_trans.
-  apply fib_iter_loop_lb2_closed_upper_bound; try omega.
-  apply (le_trans
-           (1 + n + n * plus_two_fibs_time (fb + n))
-           (64*(1+fb)*(1+n+(div2 n)*(plus_two_fibs_time (0 + div2 n)))));
-    [|apply mult_le_compat; auto;
-     apply fib_iter_loop_time_lb2_closed_lower_bound]; try omega.
-  rewrite plus_0_l.
-  repeat (rewrite mult_plus_distr_l).
-  repeat (rewrite mult_1_r).
-  repeat (rewrite plus_assoc).
-  repeat (rewrite mult_plus_distr_l).
-  repeat (rewrite mult_plus_distr_r).
-  repeat (rewrite plus_assoc).
-  eapply le_trans.
-  apply plus_le_compat.
-  apply le_refl.
-  apply mult_le_compat.
-  apply le_refl.
-  apply plus_two_fibs_time_upper_bound.
-  apply (le_trans
-           (1 + n + n * (fb + n + 4))
-           (64 + 64 * fb + 64 * n + 64 * fb * n +
-            16 * (div2 n * (div2 n)) +
-            16 * fb * (div2 n * (div2 n)))).
-  repeat (rewrite mult_plus_distr_l).
-  repeat (rewrite plus_assoc).
-  replace (1 + n + n * fb + n * n + n * 4)
-  with (1 + 5*n + n * fb + n * n);[|omega].
-  replace (64 + 64 * fb + 64 * n + 64 * fb * n + 16 * (div2 n * div2 n) +
-           16 * fb * (div2 n * div2 n))
-  with (64 + 64 * fb + 64 * n + 64 * fb * n + 16 * fb * (div2 n * div2 n) +
-        16 * (div2 n * div2 n));[|omega].
-  apply plus_le_compat.
-  replace (n*fb) with (fb*n);[|apply mult_comm].
-  repeat (rewrite <- mult_assoc).
-  remember (fb*n) as A.
-  remember (fb*(div2 n * div2 n)) as B.
-  omega.
-  replace 16 with (4*4);[|omega].
-  replace (4*4*(div2 n * div2 n)) with ((4*div2 n) *(4*div2 n)).
-  apply mult_le_compat.
-  apply mult_4_div2; omega.
-  apply mult_4_div2; omega.
-  repeat (rewrite <- mult_assoc).
-  replace (div2 n * (4*div2 n)) with ((4*div2 n)*div2 n) at 1;[|apply mult_comm].
-  repeat (rewrite mult_assoc). auto.
-  apply plus_le_compat; auto.
-  apply plus_le_compat; auto.
-  replace 64 with (16*4); try omega.
-  rewrite <- mult_assoc.
-  apply mult_le_compat; auto.
-  replace (div2 n * plus_two_fibs_time (div2 n)) with
-          (plus_two_fibs_time (div2 n) * div2 n);[|apply mult_comm].
-  rewrite mult_assoc.
-  apply mult_le_compat; auto.
-  apply plus_two_fibs_time_below.
-  replace 4 with (div2 8).
-  apply div2_monotone.
-  omega.
-  auto.
-  replace 64 with (16*4); try omega.
-  repeat (rewrite <- mult_assoc).
-  apply mult_le_compat; auto.
-  repeat (rewrite mult_assoc).
-  replace (4*fb) with (fb*4);[|apply mult_comm].
-  repeat (rewrite <- mult_assoc).
-  apply mult_le_compat; auto.
-  repeat (rewrite mult_assoc).
-  replace (4*div2 n) with (div2 n * 4);[|apply mult_comm].
-  repeat (rewrite <- mult_assoc).
-  apply mult_le_compat;auto.
-  apply plus_two_fibs_time_below.
-  replace 4 with (div2 8).
-  apply div2_monotone.
-  omega.
-  auto.
-Qed.  
-
 
 Theorem fib_iter_n_squared: big_omega fib_iter_time_lb (fun n => n * n).
 Proof.
   apply big_oh_rev.
-  destruct fib_iter_loop_time_lb3_sq as [lb3_start FACT3].
-  destruct fib_iter_loop_lb23 as [lb2_start FACT2].
-  apply (big_oh_trans (fun n=> n*n) (fun n => fib_iter_loop_time_lb3 n (max lb2_start lb3_start))).
-  apply FACT3.
-  apply Max.le_max_r.
-  clear FACT3.
-  apply (big_oh_trans (fun fuel => fib_iter_loop_time_lb3 fuel (max lb2_start lb3_start))
-                      (fun fuel => fib_iter_loop_time_lb2 fuel (max lb2_start lb3_start))).
-  apply FACT2.
-  apply Max.le_max_l.
-  clear FACT2.
-  apply (big_oh_trans (fun fuel : nat => fib_iter_loop_time_lb2 fuel (max lb2_start lb3_start))
-                      (fun fuel => fib_iter_loop_time_lb fuel 0 1));
-    [|apply fib_iter_time_lb_big_oh_fib_iter_loop_time_lb].
-  
-  remember (max lb2_start lb3_start) as fb; clear Heqfb lb3_start lb2_start.
-  destruct (fib_iter_loop_last_arg_invariant fb) as [X FACT].
-  exists 9 X.
-  intros n H.
-  replace (fib_iter_loop_time_lb n 0 1) with (fib_iter_loop_time_lb n (fib 0) (fib 1));[|unfold fib;auto].
-  rewrite fib_iter_loop_lb12.
-  apply FACT. omega.
+  apply n_squared_big_O_fib_iter_time_lb.
 Qed.
 
